Simplify the determinism proof of InterpUniv

typing.v
@@ -3,7 +3,7 @@ From Coq Require Import
   Sets.Relations_2
   ssreflect
   Program.Basics.
-From Hammer Require Import Tactics.
+From Hammer Require Import Tactics Hammer.
 
 Definition context := nat -> tm.
 
@@ -82,6 +82,20 @@ Inductive InterpUniv : tm -> (tm -> Prop) -> Prop :=
   InterpUniv A1 PA1 ->
   InterpUniv A0 PA1.
 
+Inductive InterpType : tm -> (tm -> Prop) -> Prop :=
+| InterpType_False : InterpType tFalse (const False)
+| InterpType_Fun A B PA (PF : tm -> (tm -> Prop) -> Prop) :
+  InterpType A PA ->
+  (forall a, PA a -> exists PB, PF a PB) ->
+  (forall a PB, PA a -> PF a PB -> InterpType (subst_tm (a..) B) PB) ->
+  InterpType (tPi A B) (ProdSpace PA PF)
+| InterpType_Univ :
+  InterpType tUniv (fun A => exists PA, InterpUniv A PA)
+| InterpType_Step A0 A1 PA1 :
+  Par A0 A1 ->
+  InterpType A1 PA1 ->
+  InterpType A0 PA1.
+
 Lemma InterpUniv_NotVar i P : ~ InterpUniv (var_tm i) P.
 Proof.
   move E : (var_tm i) => a0 h.
@@ -89,11 +103,25 @@ Proof.
   elim : a0 P / h; hauto inv:InterpUniv, Par.
 Qed.
 
+Lemma InterpType_NotVar i P : ~ InterpType (var_tm i) P.
+Proof.
+  move E : (var_tm i) => a0 h.
+  move : i E.
+  elim : a0 P / h; hauto inv:InterpType, Par.
+Qed.
+
 Lemma InterpUniv_NotAbs A a P : ~ InterpUniv (tAbs A a) P.
 Proof.
   move E : (tAbs A a) => a0 h.
   move : A a E.
   elim : a0 P / h; hauto inv:InterpUniv, Par.
+Qed.
+
+Lemma InterpType_NotAbs A a P : ~ InterpType (tAbs A a) P.
+Proof.
+  move E : (tAbs A a) => a0 h.
+  move : A a E.
+  elim : a0 P / h; hauto inv:InterpType, Par.
 Qed.
 
 Lemma InterpUniv_Fun_inv A0 B0 P  (h : InterpUniv (tPi A0 B0) P) :
@@ -116,6 +144,26 @@ Proof.
     hauto lq:on rew:off ctrs:InterpUniv.
 Qed.
 
+Lemma InterpType_Fun_inv A0 B0 P  (h : InterpType (tPi A0 B0) P) :
+  exists A1 B1, Rstar _ Par A0 A1 /\ Rstar _ Par B0 B1 /\ exists PA PF,
+      P = ProdSpace PA PF /\ InterpType A1 PA /\
+        (forall a PB, PA a -> PF a PB -> InterpType (subst_tm (a..) B1) PB) /\
+        (forall a, PA a -> exists PB, PF a PB).
+Proof.
+  move E : (tPi A0 B0) h => T h.
+  move : A0 B0 E.
+  elim : T P / h => //.
+  - hauto lq:on ctrs:InterpType, Rstar.
+  - move => A0 A1 PA1 h0 h1 ih A2 B2 ?; subst.
+    elim /Par_inv : h0 => //.
+    move => h2 A0 A3 B0 B1 h3 h4 [? ?] ?; subst.
+    move /(_ A3 B1 ltac:(done)) : ih.
+    intros (A1 & B3 & h5 & h6 & h7).
+    have [*] : Rstar _ Par A2 A1 /\ Rstar _ Par B2 B3
+      by hauto lq:on rew:off ctrs:Rstar use:Relations_2_facts.Rstar_transitive.
+    hauto lq:on rew:off ctrs:InterpType.
+Qed.
+
 Lemma InterpUniv_preservation A B P (h : InterpUniv A P) :
   Par A B ->
   InterpUniv B P.
@@ -135,15 +183,59 @@ Proof.
     hauto lq:on ctrs:InterpUniv.
 Qed.
 
+Lemma InterpType_preservation A B P (h : InterpType A P) :
+  Par A B ->
+  InterpType B P.
+Proof.
+  move : B.
+  elim : A P / h; auto.
+  - hauto lq:on inv:Par ctrs:InterpType.
+  - move => A B PA PF hPA ihPA hPB hPB' ihPB T hT.
+    elim /Par_inv :  hT => //.
+    move => hPar A0 A1 B0 B1 h0 h1 [? ?] ?; subst.
+    apply InterpType_Fun; auto.
+    move => a PB ha hPB0.
+    apply : ihPB; eauto.
+    sfirstorder use:par_cong, Par_refl.
+  - hauto lq:on inv:Par ctrs:InterpType.
+  - move => A B P h0 h1 ih1 C hC.
+    have [D [h2 h3]] := par_confluent _ _ _ h0 hC.
+    hauto lq:on ctrs:InterpType.
+Qed.
+
 Lemma InterpUniv_preservation_star A B P (h : InterpUniv A P) :
   Rstar _ Par A B ->
   InterpUniv B P.
 Proof. induction 1; hauto l:on use:InterpUniv_preservation. Qed.
 
+Lemma InterpType_preservation_star A B P (h : InterpType A P) :
+  Rstar _ Par A B ->
+  InterpType B P.
+Proof. induction 1; hauto l:on use:InterpType_preservation. Qed.
+
 Lemma InterpUniv_back_preservation_star A B P (h : InterpUniv B P) :
   Rstar _ Par A B ->
   InterpUniv A P.
 Proof. induction 1; hauto l:on ctrs:InterpUniv. Qed.
+
+Lemma InterpType_back_preservation_star A B P (h : InterpType B P) :
+  Rstar _ Par A B ->
+  InterpType A P.
+Proof. induction 1; hauto l:on ctrs:InterpType. Qed.
+
+Lemma InterpUniv_Fun_inv' A B P :
+  InterpUniv (tPi A B) P ->
+  exists (PA : tm -> Prop) (PF : tm -> (tm -> Prop) -> Prop),
+    InterpUniv A PA /\
+    (forall a, PA a -> exists PB, PF a PB) /\
+    (forall a PB, PA a -> PF a PB -> InterpUniv (subst_tm (a..) B) PB) /\
+    P = ProdSpace PA PF.
+Proof.
+  move /InterpUniv_Fun_inv.
+  intros (A1 & B1 & hP1 & hP2 & PA & PF & ? & hPA & hPF & hPFTotal).
+  exists PA, PF; split; eauto;
+  qauto l:on use:par_subst_star, InterpUniv_back_preservation_star.
+Qed.
 
 Lemma InterpUniv_deterministic A PA PB :
   InterpUniv A PA ->
@@ -158,30 +250,7 @@ Proof.
     move : E.
     elim : a P / h; sauto lq:on rew:off.
   - move => A B PA PF hPA ihPA hPB hPB' ihPB P hP.
-    move /InterpUniv_Fun_inv : hP.
-    intros (A1 & B1 & hP1 & hP2 & PA0 & PF0 & ? & hPA0 & hPBF0 & hPBF0'); subst.
-    move => a.
-    rewrite /ProdSpace.
-    have h0 : InterpUniv A PA0 by eauto using InterpUniv_back_preservation_star.
-    have h1 : forall a, Rstar tm Par (subst_tm (a..) B) (subst_tm (a..) B1) by sfirstorder use:par_subst_star.
-    have h2 : forall x, PA x <-> PA0 x by sfirstorder.
-    split.
-    + move => h3 a0 ha0.
-      case /(_ _ ha0) : hPBF0' => PB0 hPB0.
-      move /h2 in ha0.
-      exists PB0.
-      split; auto.
-      have ? : InterpUniv (subst_tm (a0..) B1) PB0 by sfirstorder.
-      have ? : InterpUniv (subst_tm (a0..) B) PB0 by sfirstorder use:InterpUniv_back_preservation_star.
-      qauto l:on.
-    + move => h3 a0 ha0.
-      have /h2 ha0' := ha0.
-      case /(_ _ ha0') : h3 => PB0 [hPB0 hPB0'].
-      case /(_ _ ha0) : hPB => PB1 hPB1.
-      move /(_ _ _ ha0 hPB1) in hPB'.
-      exists PB1; split; auto.
-      move /(_ a0 PB0 ha0' hPB0) in hPBF0.
-      have ? : InterpUniv (subst_tm (a0..) B) PB0 by sfirstorder use:InterpUniv_back_preservation_star.
-      qauto l:on.
+    move /InterpUniv_Fun_inv' : hP.
+    qauto l:on unfold:ProdSpace.
   - hauto l:on use:InterpUniv_preservation.
 Qed.
